src/obseq2/proof/ref.lean
@@ -13,13 +13,17 @@ theorem CompilerInv_step_ref
     {s_osea : oseair.State}
     {dst : Place Γ (obseq.LayoutTy.PtrL τ)} {src : Place Γ τ}
     (kind : RefKind)
+    (compProg : oseair.Prog)
+    (h_comp : compileProgFromChecked cs0 prog = Except.ok compProg)
     (h_inv  : CompilerInv cs0 prog ρa ρt s_mir s_osea)
     (h_stmt : prog.get? s_mir.pc = some (.assign dst (.ref kind src)))
     (h_step : obseq2.mirlite.stepStmt PermissionModel.stackedBorrows s_mir
                 (.assign dst (.ref kind src)) = .ok s_mir') :
-    ∃ (s_osea' : oseair.State) (n : Nat),
-      oseair.runN n s_osea (compileProgFrom cs0 prog) = oseair.Result.Ok s_osea' ∧
-      CompilerInv cs0 prog ρa ρt s_mir' s_osea' := by
+    ∃ (ρa' : AddrRenameMap) (ρt' : TagRenameMap) (s_osea' : oseair.State) (n : Nat),
+      AddrRenameIncr ρa ρa' ∧
+      TagRenameIncr ρt ρt' ∧
+      oseair.runN n s_osea compProg = oseair.Result.Ok s_osea' ∧
+      CompilerInv cs0 prog ρa' ρt' s_mir' s_osea' := by
   sorry
 
 end obseq2.proof
